NuLLReps.thy
@@ -1,8 +1,19 @@
 theory NuLLReps
   imports NuPrim  "HOL-Library.Word"
+  abbrevs "<own>" = "\<left_fish_tail>"
+    and "<none>" = "\<down_fish_tail>"
+    and "<object>" = "\<R_arr_tail>"
 begin
 
 text \<open>Semantic data representations\<close>
+
+section \<open>Preliminary notions\<close>
+
+datatype identity = idhypen identity nat (infixl "\<hyphen>" 70) | ID_MEM | ID_CONST string
+  \<comment> \<open>A tree-like structure allowing infinite sub identity space, like folders where infinite sub-folders can be allocated\<close>
+
+class field = lrep
+class field_list = lrep
 
 section \<open>The construction state\<close>
 
@@ -11,16 +22,125 @@ definition llty_state :: "'a state itself \<Rightarrow> llty" where [simp]: "llt
 instance by standard
 end
 
-section \<open>Miscellaneous built-in\<close>
+section \<open>Owning\<close>
+
+datatype 'a owning = Owning zint 'a (infix "\<left_fish_tail>" 60) | OwnNone ("\<down_fish_tail>")
+  \<comment> \<open>\<^term>\<open>quantity_of_ownership \<left_fish_tail> data\<close>\<close>
+
+lemma owning_forall: "All P \<longleftrightarrow> P \<down_fish_tail> \<and> (\<forall>z x. P (z \<left_fish_tail> x))" by (metis owning.exhaust) 
+lemma owning_exists: "Ex P \<longleftrightarrow> P \<down_fish_tail> \<or> (\<exists>z x. P (z \<left_fish_tail> x))" by (metis owning.exhaust) 
+
+subsection \<open>Instantiations\<close>
+
+instantiation owning :: (disposable) disposable begin
+definition disposable_owning :: " 'a owning \<Rightarrow> bool"
+  where "disposable_owning x = (case x of Owning z a \<Rightarrow> disposable a | _ \<Rightarrow> True)"
+lemma [simp]: "disposable (Owning z a) = disposable a" and [simp]: "disposable OwnNone = True"
+  unfolding disposable_owning_def by simp+
+instance by standard
+end
+
+instantiation owning :: (disposable) lrep begin
+definition llty_owning :: " 'a owning itself \<Rightarrow> llty" where "llty_owning _ = la_z"
+instance by standard
+end
+
+instantiation owning :: (disposable) field begin instance by standard end
+
+instantiation owning :: (sharing_identical) sharing_identical begin
+definition sharing_identical_owning :: " 'a owning \<Rightarrow> 'a owning \<Rightarrow> bool "
+  where "sharing_identical_owning = rel_owning sharing_identical"
+lemma [simp]: "sharing_identical (Owning z1 x1) (Owning z2 x2) \<longleftrightarrow> (z1 = z2) \<and> sharing_identical x1 x2"
+  and [simp]: "sharing_identical (Owning z1 x1) OwnNone \<longleftrightarrow> False"
+  and [simp]: "sharing_identical OwnNone (Owning z2 x2) \<longleftrightarrow> False"
+  and [simp]: "sharing_identical OwnNone OwnNone \<longleftrightarrow> True"
+  unfolding sharing_identical_owning_def by simp+
+instance proof
+  fix x y z :: \<open>'a owning\<close> and a b :: zint
+  show "sharing_identical x x" by (cases x) simp+
+  show "sharing_identical x y = sharing_identical y x" by (cases x; cases y) auto
+  show "sharing_identical x y \<Longrightarrow> sharing_identical y z \<Longrightarrow> sharing_identical x z" by (cases x; cases y; cases z) (auto intro: sharing_identical_trans)
+qed
+end
+
+instantiation owning :: (type) ownership begin
+definition ownership_owning :: " 'a owning \<Rightarrow> ownership"
+  where "ownership_owning x = (case x of Owning z _ \<Rightarrow> OWS_1 z | OwnNone \<Rightarrow> OWS_0)"
+lemma [simp]: "ownership (Owning z x) = OWS_1 z" and [simp]: "ownership OwnNone = OWS_0"
+  unfolding ownership_owning_def by simp+
+instance by standard
+end
+
+instantiation owning :: (type) share begin
+definition shareable_owning :: " 'a owning \<Rightarrow> bool " where [simp]: "shareable_owning _ = True"
+definition share_owning :: " zint \<Rightarrow> 'a owning \<Rightarrow> 'a owning "
+  where "share_owning z x = (case x of Owning z' a \<Rightarrow> Owning (z' + z) a | _ \<Rightarrow> OwnNone)"
+definition dpriv_owning :: " 'a owning \<Rightarrow> 'a owning" where [simp]: "dpriv_owning x = OwnNone"
+
+lemma [simp]: "share z (Owning z' a) = Owning (z' + z) a" and [simp]: "share z OwnNone = OwnNone"
+  unfolding share_owning_def by simp+
+
+instance proof
+  fix x y z :: \<open>'a owning\<close> and a b :: zint
+  show "share (Gi 0) x = x" by (cases x) auto
+  show "share b (share a x) = share (a + b) x" by (cases x) (auto simp add: add.assoc)
+qed
+end
+
+instantiation owning :: (type) ceq begin
+definition ceqable_owning :: " 'a owning \<Rightarrow> 'a owning \<Rightarrow> bool" where [simp]: "ceqable_owning _ _ = True"
+definition ceq_owning :: " 'a owning \<Rightarrow> 'a owning \<Rightarrow> bool" where [simp]: "ceq_owning _ _ = True"
+instance by standard auto
+end
+
+subsection \<open>Nu abstractions\<close>
+
+section \<open>Memory address\<close>
+
+datatype ('spc::len) memadr = memadr identity  \<comment> \<open>'spc : address space\<close>
+translations "id" <= "CONST memadr 0 id"
+
+lemma memadr_exisits: "Ex P \<longleftrightarrow> (\<exists>id. P (memadr id))" by (metis memadr.exhaust) 
+lemma memadr_forall: "All P \<longleftrightarrow> (\<forall>id. P (memadr id))" by (metis memadr.exhaust) 
+
+subsection \<open>Instantiations\<close>
+
+instantiation memadr :: (len) lrep begin
+definition disposable_memadr :: "'a memadr \<Rightarrow> bool" where [simp]: "disposable_memadr _ = True"
+definition llty_memadr :: "'a memadr itself \<Rightarrow> llty" where [simp]: "llty_memadr _ = la_p LENGTH('a)"
+instance by standard
+end
+
+instantiation memadr :: (len) field begin instance by standard end
+
+instantiation memadr :: (len) sharing_identical begin
+definition sharing_identical_memadr :: " 'a memadr \<Rightarrow> 'a memadr \<Rightarrow> bool" where [simp]: "sharing_identical_memadr _ _ = True"
+definition ownership_memadr :: " 'a memadr \<Rightarrow> ownership" where [simp]: "ownership_memadr _ = OWS_0"
+instance by standard auto
+end
+
+instantiation memadr :: (len) share begin
+definition shareable_memadr :: " 'a memadr \<Rightarrow> bool" where [simp]: "shareable_memadr _ = True"
+definition share_memadr :: "zint \<Rightarrow> 'a memadr \<Rightarrow> 'a memadr" where [simp]: "share_memadr z x = x"
+definition dpriv_memadr :: "'a memadr \<Rightarrow> 'a memadr" where [simp]: "dpriv_memadr x = x"
+instance by standard auto
+end
+
+instantiation memadr :: (len) naive_lrep begin
+instance by standard auto
+end
+
+section \<open>Void\<close>
 
 instantiation void :: naive_lrep begin
 definition share_void :: "zint \<Rightarrow> void \<Rightarrow> void" where [simp]: "share_void z = id"
-definition shareable_void :: "void set" where [simp]: "shareable_void = UNIV"
-definition revert_void :: "void \<Rightarrow> void \<Rightarrow> bool" where [simp]: "revert_void x y = True"
+definition shareable_void :: "void \<Rightarrow> bool" where [simp]: "shareable_void _ = True"
+definition sharing_identical_void :: "void \<Rightarrow> void \<Rightarrow> bool" where [simp]: "sharing_identical_void x y = True"
 definition dpriv_void :: "void \<Rightarrow> void" where [simp]: "dpriv_void x = x"
 instance by standard auto
 end
 
+instantiation void :: field_list begin instance by standard end
 
 section \<open>The integer data type\<close>
 
@@ -30,10 +150,11 @@ instantiation word :: (len) naive_lrep
 begin
 definition llty_word :: "'a word itself \<Rightarrow> llty" where [simp]: "llty_word _ = la_i LENGTH('a)"
 definition share_word :: "zint \<Rightarrow> 'a word \<Rightarrow> 'a word" where [simp]: "share_word z = id"
-definition shareable_word :: "'a word set" where [simp]: "shareable_word = UNIV"
-definition revert_word :: "'a word \<Rightarrow> 'a word \<Rightarrow> bool" where [simp]: "revert_word x y = True"
+definition shareable_word :: "'a word \<Rightarrow> bool" where [simp]: "shareable_word _ = True"
+definition sharing_identical_word :: "'a word \<Rightarrow> 'a word \<Rightarrow> bool" where [simp]: "sharing_identical_word x y = True"
 definition dpriv_word :: "'a word \<Rightarrow> 'a word" where [simp]: "dpriv_word x = x"
-definition disposable_word :: "'a word set" where [simp]: "disposable_word = UNIV"
+definition disposable_word :: "'a word \<Rightarrow> bool" where [simp]: "disposable_word _ = True"
+definition ownership_word :: " 'a word \<Rightarrow> ownership" where [simp]: "ownership_word _ = OWS_0"
 instance by standard auto
 end
 
@@ -43,12 +164,14 @@ definition [simp]: "lty_zero_word = (0 :: 'a word)"
 instance by standard
 end
 
-instantiation word :: (len) ceq_lrep
+instantiation word :: (len) ceq
 begin
 definition ceqable_word :: "'a word \<Rightarrow> 'a word \<Rightarrow> bool" where [simp]: "ceqable_word x y = True"
 definition ceq_word :: "'a word \<Rightarrow>  'a word \<Rightarrow> bool" where [simp]: "ceq_word x y = (x = y)"
 instance by standard (auto+)
 end
+
+instantiation word :: (len) field begin instance by standard end
 
 subsection \<open>Basic \<nu>-abstractions based on integer type\<close>
 
@@ -85,36 +208,47 @@ lemma [simp]: "p \<nuLinkL> \<bool> \<nuLinkR> x \<longleftrightarrow> (p = 1) =
 lemma [\<nu>intro]: "\<nu>CEqual \<bool> (\<lambda>x y. True)  (=)" unfolding \<nu>CEqual_def NuBool_def by auto
 
 
-section \<open>The pair abstract structure\<close>
+section \<open>Prod & the pair abstract structure\<close>
 
 subsection \<open>Lrep instantiations\<close>
+
+instantiation prod :: (field, field_list) field_list begin instance by standard end
 
 instantiation prod :: (zero_lrep, zero_lrep) zero_lrep begin
 definition lty_zero_prod :: "'a \<times> 'b" where [simp]: "lty_zero_prod = (lty_zero,lty_zero)"
 instance by standard
 end
 
-instantiation prod :: (sharable_lrep, sharable_lrep) sharable_lrep begin
-definition revert_prod :: "('a \<times> 'b) \<Rightarrow> ('a \<times> 'b) \<Rightarrow> bool"
-  where "revert_prod v1 v2 \<longleftrightarrow> (case v1 of (a1,b1) \<Rightarrow> case v2 of (a2,b2) \<Rightarrow> revert a1 a2 \<and> revert b1 b2)"
-lemma [simp]: "revert (a1,b1) (a2,b2) \<longleftrightarrow> revert a1 a2 \<and> revert b1 b2"
-  unfolding revert_prod_def by simp
-definition shareable_prod :: "('a \<times> 'b) set" where "shareable_prod = shareable \<times> shareable"
-lemma [simp]: "(a,b) \<in> shareable \<longleftrightarrow> a \<in> shareable \<and> b \<in> shareable" unfolding shareable_prod_def by simp
+instantiation prod :: (ownership, ownership) ownership begin
+definition ownership_prod :: " 'a \<times> 'b \<Rightarrow> ownership"
+  where "ownership_prod x = (case x of (a,b) \<Rightarrow> OWS_C (ownership a) (ownership b))"
+lemma [simp]: "ownership (a,b) = OWS_C (ownership a) (ownership b)" unfolding ownership_prod_def by simp
+instance by standard
+end
+
+instantiation prod :: (sharing_identical, sharing_identical) sharing_identical begin
+definition sharing_identical_prod :: "('a \<times> 'b) \<Rightarrow> ('a \<times> 'b) \<Rightarrow> bool" where "sharing_identical_prod = sharing_identical \<times>\<^sub>r sharing_identical"
+lemma [simp]: "sharing_identical (a1,b1) (a2,b2) \<longleftrightarrow> sharing_identical a1 a2 \<and> sharing_identical b1 b2"
+  unfolding sharing_identical_prod_def by simp
+instance by standard (auto intro: sharing_identical_trans)
+end
+
+instantiation prod :: (share, share) share begin
+definition shareable_prod :: "('a \<times> 'b) \<Rightarrow> bool" where "shareable_prod = shareable \<times>\<^sub>p shareable"
 definition share_prod :: "zint \<Rightarrow> 'a \<times> 'b \<Rightarrow> 'a \<times> 'b" where [simp]: "share_prod z x = (case x of (a,b) \<Rightarrow> (share z a, share z b))"
 definition dpriv_prod :: "'a \<times> 'b \<Rightarrow> 'a \<times> 'b" where [simp]: "dpriv_prod x = (case x of (a,b) \<Rightarrow> (dpriv a, dpriv b))"
-instance by standard (auto intro: revert_trans)
+lemma [simp]: "shareable (a,b) \<longleftrightarrow> shareable a \<and> shareable b" unfolding shareable_prod_def by simp
+instance by standard auto
 end
 
 instantiation prod :: (naive_lrep, naive_lrep) naive_lrep
   begin instance by standard auto end
 
-instantiation prod :: (ceq_lrep, ceq_lrep) ceq_lrep begin
-definition ceqable_prod :: "'a \<times> 'b \<Rightarrow> 'a \<times> 'b \<Rightarrow> bool"
-  where "ceqable_prod x y = (case x of (a1,b1) \<Rightarrow> case y of (a2,b2) \<Rightarrow> ceqable a1 a2 \<and> ceqable b1 b2)"
+instantiation prod :: (ceq, ceq) ceq begin
+definition ceqable_prod :: "'a \<times> 'b \<Rightarrow> 'a \<times> 'b \<Rightarrow> bool" where "ceqable_prod  = ceqable \<times>\<^sub>r ceqable"
 lemma [simp]: "ceqable (a1,b1) (a2,b2) \<longleftrightarrow> ceqable a1 a2 \<and> ceqable b1 b2" unfolding ceqable_prod_def by auto
-definition ceq_prod :: "'a \<times> 'b \<Rightarrow> 'a \<times> 'b \<Rightarrow> bool"
-  where [simp]: "ceq_prod x y = (case x of (a1,b1) \<Rightarrow> case y of (a2,b2) \<Rightarrow> ceq a1 a2 \<and> ceq b1 b2)"
+definition ceq_prod :: "'a \<times> 'b \<Rightarrow> 'a \<times> 'b \<Rightarrow> bool" where "ceq_prod = ceq \<times>\<^sub>r ceq"
+lemma [simp]: "ceq (a1,b1) (a2,b2) \<longleftrightarrow> ceq a1 a2 \<and> ceq b1 b2" unfolding ceq_prod_def by auto
 instance by standard (auto intro: ceq_trans)
 end
 
@@ -122,63 +256,181 @@ subsection \<open>Fusion \<nu>-abstraction\<close>
 
 definition Fusion :: "('a1::lrep,'b1) nu \<Rightarrow> ('a2::lrep,'b2) nu \<Rightarrow> ('a1 \<times> 'a2, 'b1 \<times> 'b2) nu" (infixr "\<nuFusion>" 70) 
   where "Fusion N M = Nu (\<lambda>px. case px of ((p1,p2),(x1,x2)) \<Rightarrow> (p1 \<nuLinkL> N \<nuLinkR> x1) \<and> (p2 \<nuLinkL> M \<nuLinkR> x2))"
-lemma Fusion_abst[simp]: "(p1,p2) \<nuLinkL> N \<nuFusion> M \<nuLinkR> (x1,x2) \<longleftrightarrow> (p1 \<nuLinkL> N \<nuLinkR> x1) \<and> (p2 \<nuLinkL> M \<nuLinkR> x2)"
-  unfolding Fusion_def by simp
-lemma "Inhabited \<tort_lbrace>(x1,x2) \<tycolon> N1 \<nuFusion> N2\<tort_rbrace> \<longleftrightarrow> Inhabited \<tort_lbrace>x1 \<tycolon> N1\<tort_rbrace> \<and> Inhabited \<tort_lbrace>x2 \<tycolon> N2\<tort_rbrace>"
-  unfolding Inhabited_def by simp
 
-lemma [\<nu>intro]: "\<nu>Share N s1 f1 \<Longrightarrow> \<nu>Share M s2 f2 \<Longrightarrow> \<nu>Share (N \<nuFusion> M) (s1 \<times> s2) (\<lambda>z x. case x of (x1,x2) \<Rightarrow> (f1 z x1, f2 z x2))"
-  for N :: "('a :: sharable_lrep, 'b) nu" and M :: "('c :: sharable_lrep, 'd) nu" 
-  unfolding \<nu>Share_def by auto
-lemma [\<nu>intro]: "\<nu>CEqual N p \<Longrightarrow> \<nu>CEqual M q \<Longrightarrow> \<nu>CEqual (N \<nuFusion> M) (\<lambda>x. case x of ((a1,b1),(a2,b2)) \<Rightarrow> p (a1,a2) \<and> q (b1,b2))"
-  unfolding \<nu>CEqual_def by auto
+lemma [simp]: "(p1,p2) \<nuLinkL> N \<nuFusion> M \<nuLinkR> (x1,x2) \<longleftrightarrow> (p1 \<nuLinkL> N \<nuLinkR> x1) \<and> (p2 \<nuLinkL> M \<nuLinkR> x2)" unfolding Fusion_def by simp
+lemma [elim]: "(x1,x2) \<ratio> N1 \<nuFusion> N2 \<Longrightarrow> (x1 \<ratio> N1 \<Longrightarrow> x2 \<ratio> N2 \<Longrightarrow> C) \<Longrightarrow> C" unfolding Inhabited_def by simp
 
-lemma [\<nu>intro]: "\<nu>Disposable \<tort_lbrace>x \<tycolon> X\<tort_rbrace> \<Longrightarrow> \<nu>Disposable \<tort_lbrace>y \<tycolon> Y\<tort_rbrace> \<Longrightarrow> \<nu>Disposable \<tort_lbrace>(x,y) \<tycolon> X \<nuFusion> Y\<tort_rbrace>"
-  unfolding \<nu>Disposable_def by auto
-
+lemma [\<nu>intro]: "\<nu>Share N s1 f1 \<Longrightarrow> \<nu>Share M s2 f2 \<Longrightarrow> \<nu>Share (N \<nuFusion> M) (s1 \<times>\<^sub>p s2) (\<lambda>z. map_prod (f1 z) (f2 z))" unfolding \<nu>Share_def by auto
+lemma [\<nu>intro]: "\<nu>CEqual N P eq1 \<Longrightarrow> \<nu>CEqual M Q eq2 \<Longrightarrow> \<nu>CEqual (N \<nuFusion> M) (P \<times>\<^sub>r Q) (eq1 \<times>\<^sub>r eq2)"unfolding \<nu>CEqual_def pair_forall by auto
+lemma [\<nu>intro]: "\<nu>Disposable \<tort_lbrace>x \<tycolon> X\<tort_rbrace> \<Longrightarrow> \<nu>Disposable \<tort_lbrace>y \<tycolon> Y\<tort_rbrace> \<Longrightarrow> \<nu>Disposable \<tort_lbrace>(x,y) \<tycolon> X \<nuFusion> Y\<tort_rbrace>" unfolding \<nu>Disposable_def pair_forall by auto
+lemma [\<nu>intro]: "\<nu>ShrIdentical N sid1 \<Longrightarrow> \<nu>ShrIdentical M sid2 \<Longrightarrow> \<nu>ShrIdentical (N \<nuFusion> M) (sid1 \<times>\<^sub>r sid2)" unfolding \<nu>ShrIdentical_def by (auto 0 4)
 
 section \<open>Tuple\<close>
 
-class field = lrep
-class field_list = lrep
-
-instantiation void :: field_list begin instance by standard end
-instantiation prod :: (field, field_list) field_list begin instance by standard end
-instantiation word :: (len) field begin instance by standard end
-
 datatype 'a tuple = Tuple "('a::field_list)"
+
+lemma tuple_exists: "Ex P \<longleftrightarrow> (\<exists>x. P (Tuple x))" by (metis tuple.exhaust) 
+lemma tuple_forall: "All P \<longleftrightarrow> (\<forall>x. P (Tuple x))" by (metis tuple.exhaust) 
 
 subsection \<open>Lrep instantiations\<close>
 
+subsubsection \<open>lrep\<close>
+
 instantiation tuple :: (field_list) lrep begin
 definition llty_tuple :: " 'a tuple itself \<Rightarrow> llty " where [simp]: "llty_tuple _ = la_tup (llty TYPE('a))"
-definition disposable_tuple :: " 'a tuple set " where [simp]: "disposable_tuple = image Tuple disposable"
+definition disposable_tuple :: " 'a tuple \<Rightarrow> bool " where "disposable_tuple = pred_tuple disposable"
+lemma [simp]: "disposable (Tuple x) = disposable x" unfolding disposable_tuple_def by simp
 instance by standard
 end
+
+subsubsection \<open>zero\<close>
 
 instantiation tuple :: ("{zero_lrep,field_list}") zero_lrep begin
 definition lty_zero_tuple :: " 'a tuple " where [simp]: "lty_zero_tuple = Tuple lty_zero"
 instance by standard
 end
 
-instantiation tuple :: ("{sharable_lrep,field_list}") sharable_lrep begin
-definition shareable_tuple :: " 'a tuple set " where [simp]: "shareable_tuple = image Tuple shareable"
-definition share_tuple :: " zint \<Rightarrow> 'a tuple \<Rightarrow> 'a tuple " where [simp]: "share_tuple z = map_tuple (share z)"
-definition revert_tuple :: " 'a tuple \<Rightarrow> 'a tuple \<Rightarrow> bool " where "revert_tuple x y = (case x of Tuple a \<Rightarrow> case y of Tuple b \<Rightarrow> revert a b)"
-lemma [simp]: "revert (Tuple a) (Tuple b) \<longleftrightarrow> revert a b" unfolding revert_tuple_def by simp
-definition dpriv_tuple :: " 'a tuple \<Rightarrow> 'a tuple " where "dpriv_tuple = map_tuple dpriv"
+subsubsection \<open>shareable\<close>
+
+instantiation tuple :: ("{ownership,field_list}") ownership begin
+definition ownership_tuple :: " 'a tuple \<Rightarrow> ownership" where "ownership_tuple = case_tuple ownership"
+lemma [simp]: "ownership (Tuple a) = ownership a" unfolding ownership_tuple_def by simp
+instance by standard
+end
+
+instantiation tuple :: ("{sharing_identical,field_list}") sharing_identical begin
+definition sharing_identical_tuple :: " 'a tuple \<Rightarrow> 'a tuple \<Rightarrow> bool " where "sharing_identical_tuple = rel_tuple sharing_identical"
+lemma [simp]: "sharing_identical (Tuple a) (Tuple b) \<longleftrightarrow> sharing_identical a b" unfolding sharing_identical_tuple_def by simp
 instance proof
   fix x y z :: " 'a tuple"  and a b :: zint
-  show "revert x x" by (cases x) auto
-  show "revert x y = revert y x" by (cases x, cases y) (auto simp add: revert_sym)
-  show "revert x y \<Longrightarrow> revert y z \<Longrightarrow> revert x z" by (cases x, cases y, cases z) (auto intro: revert_trans)
+  show "sharing_identical x x" by (cases x) simp
+  show "sharing_identical x y = sharing_identical y x" by (cases x, cases y) simp
+  show "sharing_identical x y \<Longrightarrow> sharing_identical y z \<Longrightarrow> sharing_identical x z" by (cases x, cases y, cases z) (auto intro: sharing_identical_trans)
+qed
+end
+
+instantiation tuple :: ("{share,field_list}") share begin
+definition shareable_tuple :: " 'a tuple \<Rightarrow> bool " where [simp]: "shareable_tuple = pred_tuple shareable"
+definition share_tuple :: " zint \<Rightarrow> 'a tuple \<Rightarrow> 'a tuple " where [simp]: "share_tuple z = map_tuple (share z)"
+definition dpriv_tuple :: " 'a tuple \<Rightarrow> 'a tuple " where "dpriv_tuple = map_tuple dpriv"
+lemma [simp]: "shareable (Tuple x) = shareable x" unfolding shareable_tuple_def by simp
+lemma [simp]: "share z (Tuple x) = Tuple (share z x)" unfolding share_tuple_def by simp
+lemma [simp]: "dpriv (Tuple a) = Tuple (dpriv a)" unfolding dpriv_tuple_def by simp
+instance proof
+  fix x y z :: " 'a tuple"  and a b :: zint
   show "share (Gi 0) x = x" by (cases x) auto
   show "share b (share a x) = share (a + b) x" by (cases x) auto
 qed
 end
 
-term "(O)"
-instantiation tuple :: ("{ceq_lrep,field_list}") ceq_lrep begin
+subsubsection \<open>ceq\<close>
 
+instantiation tuple :: ("{ceq,field_list}") ceq begin
+definition ceqable_tuple :: " 'a tuple \<Rightarrow> 'a tuple \<Rightarrow> bool " where "ceqable_tuple = rel_tuple ceqable"
+definition ceq_tuple :: " 'a tuple \<Rightarrow> 'a tuple \<Rightarrow> bool " where "ceq_tuple = rel_tuple ceq"
+lemma [simp]: "ceqable (Tuple a) (Tuple b) = ceqable a b" unfolding ceqable_tuple_def by simp
+lemma [simp]: "ceq (Tuple a) (Tuple b) = ceq a b" unfolding ceq_tuple_def by simp
+instance proof
+  fix x y z :: " 'a tuple"
+  show "ceqable x y = ceqable y x" by (cases x; cases y) simp
+  show "ceqable x x \<Longrightarrow> ceq x x" by (cases x) auto
+  show "ceqable x y \<Longrightarrow> ceq x y = ceq y x" by (cases x; cases y) simp
+  show "ceqable x y \<Longrightarrow> ceqable y z \<Longrightarrow> ceqable x z \<Longrightarrow> ceq x y \<Longrightarrow> ceq y z \<Longrightarrow> ceq x z" by (cases x, cases y, cases z) (simp, blast intro: ceq_trans)
+qed
 end
+
+subsubsection \<open>naive\<close>
+
+instantiation tuple :: ("{naive_lrep,field_list}") naive_lrep begin
+instance proof
+  fix x y :: " 'a tuple " and z :: zint
+  show "disposable x = True" by (cases x) simp
+  show "shareable x = True" by (cases x) simp
+  show "dpriv x = x" by (cases x) simp
+  show " share z x = x" by (cases x) simp
+  show " sharing_identical x y = True" by (cases x; cases y) simp
+qed
+end
+
+subsubsection \<open>miscellaneous\<close>
+
+instantiation tuple :: (field_list) field begin instance by standard end
+
+subsection \<open>Nu abstraction - `NuTuple`\<close>
+
+definition NuTuple :: "(('a::field_list), 'b) nu \<Rightarrow> ('a tuple, 'b) nu" ("\<lbrace> _ \<rbrace>")
+  where "\<lbrace> N \<rbrace> = Nu (\<lambda>(p,x). case p of Tuple p' \<Rightarrow> p' \<nuLinkL> N \<nuLinkR> x)"
+
+lemma [simp]: "Tuple p \<nuLinkL> \<lbrace> N \<rbrace> \<nuLinkR> x \<longleftrightarrow> p \<nuLinkL> N \<nuLinkR> x" unfolding NuTuple_def by simp
+lemma [elim]: "x \<ratio> \<lbrace> N \<rbrace> \<Longrightarrow> (x \<ratio> N \<Longrightarrow> C) \<Longrightarrow> C" unfolding Inhabited_def tuple_exists by simp
+
+lemma [\<nu>intro]: "\<nu>Share N s f \<Longrightarrow> \<nu>Share \<lbrace> N \<rbrace> s f" unfolding \<nu>Share_def tuple_forall by simp
+lemma [\<nu>intro]: "\<nu>CEqual N P eq \<Longrightarrow> \<nu>CEqual \<lbrace> N \<rbrace> P eq" unfolding \<nu>CEqual_def tuple_forall by simp
+lemma [\<nu>intro]: "\<nu>Disposable \<tort_lbrace>x \<tycolon> X\<tort_rbrace> \<Longrightarrow> \<nu>Disposable \<tort_lbrace>x \<tycolon> \<lbrace> X \<rbrace>\<tort_rbrace>" unfolding \<nu>Disposable_def tuple_forall by simp
+lemma [\<nu>intro]: "\<nu>ShrIdentical N sid \<Longrightarrow> \<nu>ShrIdentical \<lbrace> N \<rbrace> sid" unfolding \<nu>ShrIdentical_def tuple_forall by simp
+
+section \<open>Memory Witness\<close>
+
+datatype ('len::len, 'a::field) memcon = memcon \<open>('len::len) memadr\<close> \<open>'a::field\<close>
+type_synonym ('len,'a) memobj = " ('len,'a) memcon owning"
+
+lemma memcon_forall: "All P \<longleftrightarrow> (\<forall>a x. P (memcon a x))" by (metis memcon.exhaust) 
+lemma memcon_exists: "Ex P \<longleftrightarrow> (\<exists>a x. P (memcon a x))" by (metis memcon.exhaust) 
+
+
+subsection \<open>Instantiations\<close>
+
+instantiation memcon :: (len,field) disposable begin
+definition disposable_memcon :: " ('a,'b) memcon \<Rightarrow> bool" where [simp]: "disposable_memcon _ = False"
+instance by standard
+end
+
+instantiation memcon :: ("len", "{ownership, field}") ownership begin
+definition ownership_memcon :: " ('a,'b) memcon \<Rightarrow> ownership"
+  where "ownership_memcon x = (case x of memcon _ y \<Rightarrow> ownership y)"
+lemma [simp]: "ownership (memcon p x) = ownership x"
+  unfolding ownership_memcon_def by simp
+instance by standard
+end
+
+instantiation memcon :: ("len", "{sharing_identical,ownership, field}") sharing_identical begin
+definition sharing_identical_memcon :: "  ('a,'b) memcon \<Rightarrow> ('a,'b) memcon \<Rightarrow> bool"
+  where "sharing_identical_memcon = rel_memcon (=) (inv_imagep (=) ownership)"
+lemma [simp]: "sharing_identical (memcon pa a) (memcon pb b) \<longleftrightarrow> (pa = pb) \<and> (ownership a = ownership b)"
+  unfolding sharing_identical_memcon_def by (cases pa; cases pb) simp
+instance proof
+  fix x y z :: " ('a,'b) memcon"
+  show "sharing_identical x x" by (cases x) simp
+  show "sharing_identical x y = sharing_identical y x" by (cases x; cases y) auto
+  show "sharing_identical x y \<Longrightarrow> sharing_identical y z \<Longrightarrow> sharing_identical x z" by (cases x; cases y; cases z) auto
+qed
+end
+
+subsection \<open>\<nu>-abstraction\<close>
+
+datatype 'a object = object identity 'a (infix "\<R_arr_tail>" 62)
+
+lemma object_forall: "All P \<longleftrightarrow> (\<forall>a x. P (a \<R_arr_tail> x))" by (metis object.exhaust)
+lemma object_exists: "Ex P \<longleftrightarrow> (\<exists>a x. P (a \<R_arr_tail> x))" by (metis object.exhaust)
+
+
+definition MemObj :: "(('a::field), 'b) nu \<Rightarrow> ((('len::len),'a) memobj, 'b object owning) nu"
+  where "MemObj N = Nu (\<lambda>px.
+    case px of (zp \<left_fish_tail> memcon (memadr adrp) p , z \<left_fish_tail> (adrx \<R_arr_tail> x)) \<Rightarrow> (zp = z) \<and> (adrp = adrx) \<and> (p \<nuLinkL> N \<nuLinkR> x)
+        | (\<down_fish_tail> , \<down_fish_tail>) \<Rightarrow> True | _ \<Rightarrow> False)"  
+
+lemma [simp]: "zp \<left_fish_tail> memcon (memadr  adrp) p \<nuLinkL> MemObj N \<nuLinkR> z \<left_fish_tail> adrx \<R_arr_tail> x \<longleftrightarrow> (zp = z) \<and> (adrp = adrx) \<and> (p \<nuLinkL> N \<nuLinkR> x)"
+  and [simp]: "\<down_fish_tail> \<nuLinkL> MemObj N \<nuLinkR> x' \<longleftrightarrow> x' = \<down_fish_tail>" and [simp]: "p' \<nuLinkL> MemObj N \<nuLinkR> \<down_fish_tail> \<longleftrightarrow> p' = \<down_fish_tail>"
+  unfolding MemObj_def by  (auto simp add: memadr_forall split: memcon.split owning.split)
+
+lemma [\<nu>intro]: "\<nu>Share (MemObj N) (\<lambda>x. True) share"
+  unfolding \<nu>Share_def by (simp add: owning_forall memcon_forall memadr_forall object_forall)
+lemma [\<nu>intro]: "\<nu>Disposable \<tort_lbrace>\<down_fish_tail> \<tycolon> MemObj N\<tort_rbrace>" unfolding \<nu>Disposable_def by simp
+lemma [\<nu>intro]: "\<nu>CEqual (MemObj N) (\<lambda>x y. True) (\<lambda>x y. True)" unfolding \<nu>CEqual_def by simp
+lemma [\<nu>intro]: "\<nu>Ownership (MemObj N) ownership"
+  unfolding \<nu>Ownership_def by (simp add: owning_forall memcon_forall memadr_forall object_exists)
+lemma [\<nu>intro]: "\<nu>Ownership N ow \<Longrightarrow> \<nu>ShrIdentical (MemObj N) (rel_owning (rel_object (inv_imagep (=) ow)))"
+  unfolding \<nu>Ownership_def \<nu>ShrIdentical_def
+  by (simp add: owning_forall memcon_forall memadr_forall object_exists owning_exists) auto
+
 end
